# Polar Coordinates

Instead of (x, y), we use [r, θ] for distance from the origin and anticlockwise angle from the x-axis.

## Overview

- Understand how Cartesian coordinates and polar coordinates are related
- Find the polar form of a curve given in Cartesian form
- Recognise some conics given in polar form

## Polar Coordinates

In polar coordinates, a point is represented by the ordered pair [r, θ]. Note the square brackets, to 
distinguish from the Cartesian coordinates (x, y).

These forms can be converted to each other using the following equations:
```math
r = +\sqrt{x^2 + y^2}
\tan(\theta) = \frac{y}{x}

x = r \cos(\theta)
y = r \sin(\theta)
```
The angle θ is measured anticlockwise from the positive x-axis, typically in radians. The distance r is 
the distance from the origin to the point and is positive.

Note that the fact that `$\tan(\theta) = y/x$` does NOT mean that `$\theta = \tan^{-1}(y/x)$`. 
This is because the tangent function is periodic, and this would make it seem like theta only
lies in the 1st and 4th quadrants (to the right of the y-axis).

The line from (x, y) to the origin will make an angle of `$\tan^{-1}(y/x)$` with the x-axis, but
it may not be accurate to which _direction_ in the line the point is. For example, the point (-1, 1)
is in the 2nd quadrant (top-left), but `$\tan^{-1}(1/-1)$` is in the 4th quadrant (bottom-right).

We use polar coordinates because some problems are easier to solve in polar coordinates than in Cartesian 
coordinates, especially circles - its literally just `$r=a$` for a circle with radius `$a$`.

## Finding Polar Coordinate Forms

### Circle Example

To find the polar coordinate form of a circle:
```math
x^2 + y^2 = 1
```
We then substitute `$x$` and `$y$` with their polar equivalents:
```math
(r \cos(\theta))^2 + (r \sin(\theta))^2 = 1
r^2 (\cos^2(\theta) + \sin^2(\theta)) = 1
r^2 = 1
```
Which makes sense because its a circle with radius 1.

### Parabola Example

To find the polar coordinate form of a parabola:
```math
y=2x^2
```

Note: This is an upwards parabola, not a sideways one. `$a$` here is `$1/8$`, not `$1/2$`.

We substitute and get:
```math
r \sin(\theta) = 2(r \cos(\theta)^2)^2
r \sin(\theta) - 2r^2\cos(\theta)^2 = 0
r(\sin(\theta) - 2r\cos(\theta)^2) = 0
```
Either `$r = 0$`, which is obviously false as that would be a point, not a parabola, or:
```math
\sin(\theta) - 2r\cos(\theta)^2 = 0
2r\cos(\theta)^2 = -\sin(\theta)
r = \frac{1}{2} \tan(\theta) \sec(\theta)
```

A slightly more complicated example is:
```math
y^2 = 1 + 2x
```
Unlike the previous example, this does not start at the origin. Substituting gives:
```math
(r \sin(\theta))^2 = 1 + 2(r \cos(\theta))
r^2 \sin^2(\theta) - 2r \cos(\theta) - 1 =
r^2 \sin^2(\theta) + r(-2\cos(\theta)) - 1 = 0
```
We can then use the quadratic formula to solve for r: (we only consider the positive root, as the parabola is on the 
positive side of the y-axis)
```math
r = \frac{2\cos(\theta) + \sqrt{(-2\cos(\theta))^2 - 4(\sin^2(\theta))(-1)}}{2\sin^2(\theta)}

= \frac{2\cos(\theta) + \sqrt{4\cos^2(\theta) + 4\sin^2(\theta)}}{2\sin^2(\theta)}

= \frac{2\cos(\theta) + 2}{{2\sin^2(\theta)}}

= \frac{\cos(\theta) + 1}{\sin^2(\theta)}

= \frac{\cos(\theta) + 1}{1 - \cos^2(\theta)}

= \frac{\cos(\theta) + 1}{(1 - \cos(\theta))(1 + \cos(\theta))}

= \frac{1}{1 - \cos(\theta)}
```

### Line Example

For a line which passes through the origin, we can use the polar form:
```math
y = mx
\theta = \tan^{-1}(m)
```

But for a line which does not pass through the origin, it is a bit more complicated:
```math
y = mx + c
r \sin(\theta) = m(r \cos(\theta)) + c
r \sin(\theta) - mr \cos(\theta) = c
r(\sin(\theta) - m \cos(\theta)) = c
r = \frac{c}{\sin(\theta) - m \cos(\theta)}
```

## Finding Cartesian Forms

For example,
```math
r = \cos(\theta)
```
We can multiply both sides by r to get:
```math
r^2 = r \cos(\theta)
```
Notice that `$r \cos(\theta) = x$`. We can then substitute:
```math
r^2 = x
sqrt(x^2 + y^2)^2 = x
x^2 + y^2 = x
x^2 - x + y^2 = 0
```
Completing the square gives:
```math
(x - \frac{1}{2})^2 - (\frac{1}{2})^2 + y^2 = 0
(x - \frac{1}{2})^2 + y^2 = (\frac{1}{2})^2 = \frac{1}{4}
```
So we get a circle with center `$(1/2, 0)$` and radius `$1/2$`.

## Generic Conics with Polar Coordinates

A conic is defined as the set of points on a plane such that the ratio of the distance from a point to a focus and 
the distance from the point to a directrix is the eccentricity `$e$` of the conic. That is:
```math
\frac{\textrm{distance from point to focus}}{\textrm{perpendicular distance from point to directrix}} = e
```

In particular, if
- `$e<1$`, it is an ellipse
- `$e=1$`, it is a parabola
- `$e>1$`, it is a hyperbola

@Image(source: "Graph_Conic Section Polar Derivation", alt: "Conic")

We can derive the polar form of a conic from this definition:
```math
\frac{\textrm{distance from point to focus}}{\textrm{perpendicular distance from point to directrix}} = e

\frac{r}{d+r\cos(\theta)} = e

r = e(d + r\cos(\theta))
```

Solving for r gives:
```math
r = ed + re\cos(\theta)
r - re\cos(\theta) = ed
r(1 - e\cos(\theta)) = ed
r = \frac{ed}{1 - e\cos(\theta)}
```

By definition, one of the foci is at the origin. Note that the foci will be horizontal, since 
`$\cos(y)$` is the same for a point P and its reflection across the y-axis.

### Inspecting the Conic

We know that when `$e = 0$`, the conic is a circle. You can see this from the polar form:
```math
r = \frac{0}{1 - 0\cos(\theta)} = 0
```
This is a point at the origin, which is a circle with radius 0.

When `$0 < e < 1$`, the conic is an ellipse. Inspecting the polar form:
```math
r = \frac{ed}{1 - e\cos(\theta)}
```
In this case, `$1 - e\cos(\theta) > 0$` since `$e\cos(\theta) < 1$`.