# Trigonometric Identities

When two trigonometric functions are equal for all values of variables

## Overview

- use the main trigonometric identities
- use trigonometric identities to combine trigonometric functions

All the important trigo identities are in the formula sheet.

Note that you CANNOT prove a trigonometric identity by substituting values for the variables, since that 
only proves that the functions are equal for those specific values. You must prove it for all values, by 
manipulating one side to become the other.

## Identities

Repeating the identities from <doc:Trig-functions-identities-and-equations#Identities>:

Quotient identity:
```math
\tan(\theta) \equiv \frac{sin(\theta)}{cos(\theta)}
```

Reciprocal identities:
```math
\cosec(\theta) \equiv \frac{1}{\sin(\theta)}
\sec(\theta) \equiv \frac{1}{\cos(\theta)}
\cot(\theta) \equiv \frac{1}{\tan(\theta)}
```

Pythagoras identity:
```math
\sin^2(\theta) + \cos^2(\theta) \equiv 1
\tan^2(\theta) + 1 \equiv \sec^2(\theta)
1 + \cot^2(\theta) \equiv \cosec^2(\theta)
```

Addition formulae:
```math
\sin(A \pm B) = \sin(A)\cos(B) \pm \cos(A)\sin(B)
\cos(A \pm B) = \cos(A)\cos(B) \mp \sin(A)\sin(B)

\tan(A \pm B) = \frac{\tan(A) \pm \tan(B)}{1 \mp \tan(A)\tan(B)}
```

Double angle formulae:
```math
\sin(2A) = 2 \sin(A)\cos(A)
\cos(2A) = \cos^2(A) - \sin^2(A) 
\quad = 2\cos^2(A) - 1 
\quad = 1 - 2\sin^2(A)

\tan(2A) = \frac{2\tan(A)}{1 - \tan^2(A)}
```

Triple angle formulae:
```math
\cos3A = 4 \cos^3 A - 3\cos A
\sin 3A = 3\sin A - 4\sin^3 A

\tan3A = \dfrac{3\tan A - 3\cos A}{1-3\tan^2 A}
```

See <doc:Trig-functions-identities-and-equations#Useful-Relationships> for relationships like `$sin(90 - \theta)$` etc.

Theres also the sum of sines/cosines formula.
```math
\sin(A) + \sin(B) = 2\sin\left(\frac{A+B}{2}\right)\cos\left(\frac{A-B}{2}\right)

\cos(A) + \cos(B) = 2\cos\left(\frac{A+B}{2}\right)\cos\left(\frac{A-B}{2}\right)
```

### Deriving Sum of Sines and Cosines Formula
Given these two identities:
```math
\sin(A + B) = \sin(A)\cos(B) + \cos(A)\sin(B)
\sin(A - B) = \sin(A)\cos(B) - \cos(A)\sin(B)
```

Adding them gives:
```math
\sin(A + B) + \sin(A - B) = 2\sin(A)\cos(B)
```

We can now define `$C = A + B$` and `$D = A - B$`, so that
```math
A = \frac{C + D}{2} \quad \textrm{and} \quad B = \frac{C - D}{2}
```

Hence, we can write the sum of two sines as:
```math
\sin(A) + \sin(B) = 2\sin\left(\frac{A+B}{2}\right)\cos\left(\frac{A-B}{2}\right)
```

The derivation for subtraction of sines and addition/subtraction of cosines is pretty similar, with
different things canceling out.

## Using Identities

Identities are used to either
- Simplify expressions
- Prove that two expressions are equal, by manipulating one side to become the other

We use the triple-equals sign `$\equiv$` to denote that two expressions are equal for all values of the 
variables. Note that it is valid to say that, when `$A \equiv B$`, that `$A = B$`. DO NOT do the opposite.